splitting Records.fst into three test cases

pulse/share/steel/examples/pulse/bug-reports/Records.fst
@@ -1,17 +1,11 @@
 module Records
-open Pulse.Steel.Wrapper
-module R = Steel.ST.Reference
-module A = Steel.ST.Array
 open Steel.FractionalPermission
 open FStar.Ghost
-module U8 = FStar.UInt8
-module US = FStar.SizeT
-module PM = Pulse.Main
-module T = FStar.Tactics
-module PM = Pulse.Main
-open Steel.ST.Util 
 open Pulse.Steel.Wrapper
-
+open Steel.ST.Util 
+module R = Steel.ST.Reference
+module U8 = FStar.UInt8
+module PM = Pulse.Main
 
 (* test record mutation and permissions for records of byte refs *)
 
@@ -26,21 +20,49 @@ type rec_repr = {
   v2: U8.t;
 }
 
-(* defining rec_perm directly cause Core to prove `v.v1 == u.v1` by proving `v == u` which is bad.
-  This indirection prevents F* from unfolding it and that works around the problem.
-  Should fix this in Core.
-*)
-assume
-val rec_perm (r:rec2) (v:rec_repr)
+let rec_perm (r:rec2) (v:rec_repr)
   : vprop
+  = R.pts_to r.r1 full_perm v.v1 `star`
+    R.pts_to r.r2 full_perm v.v2
 
-assume
-val rec_perm_definition (r:rec2) (v:rec_repr)
-  : Lemma 
-    (ensures rec_perm r v == 
-      (R.pts_to r.r1 full_perm v.v1 `star`
-       R.pts_to r.r2 full_perm v.v2))
-    [SMTPat (rec_perm r v)]
+//Using record syntax directly in Pulse vprops
+//leads to strange type inference errors
+let mk_rec_repr (v1 v2:U8.t) = { v1=v1; v2=v2 }
+
+
+// When defining a predicate like rec_perm relating 
+// a record and a record_repr, it's convenient to define
+// a ghost function to fold the predicate.
+// Eventually, it would be nice to auto-generate this 
+// ghost function from the predicate definition.
+```pulse
+ghost
+fn fold_rec_perm (r:rec2) (#v1 #v2:erased U8.t)
+  requires
+    R.pts_to r.r1 full_perm v1 **
+    R.pts_to r.r2 full_perm v2
+  ensures
+    rec_perm r (mk_rec_repr v1 v2)
+{
+  fold (rec_perm r (mk_rec_repr v1 v2))
+}
+```
+
+// Then, mutating a single field of the record involves:
+```pulse
+fn mutate_r2 (r:rec2) (#v:Ghost.erased rec_repr)
+  requires rec_perm r v
+  ensures exists (v_:rec_repr) .
+    rec_perm r v_ ** pure (v_.v2 == 0uy /\ v_.v1 == v.v1)
+{
+  unfold (rec_perm r v); //1. unfolding the predicate
+  r.r2 := 0uy;           //2. working with the fields
+  fold_rec_perm r;       //3. folding it back up
+  ()
+}
+```
+
+//Some alternate ways to do it, useful test cases
 
 // helpers 
 
@@ -55,32 +77,13 @@ ensures R.pts_to x full_perm y ** pure (y==z)
 ```
 
 ```pulse
-fn mutate_ref (r:R.ref U8.t) (x:U8.t) (#v:Ghost.erased U8.t)
-  requires R.pts_to r full_perm v
-  ensures R.pts_to r full_perm x
-{
-  r := x;
-  ()
-}
-```
-
-
-// this works without the introduction, but pulse can't 
-// infer the existential unless v is provided as a witness
-// and fails with a mysterious error: "match_typ: t2 is a uvar"
-[@@expect_failure]
-```pulse
-fn rec_get_witness (r:rec2) (#v:Ghost.erased rec_repr)
+fn unfold_and_fold_manually (r:rec2) (#v:Ghost.erased rec_repr)
   requires rec_perm r v
   ensures exists (v_:rec_repr) . rec_perm r v_
 {
   rewrite (rec_perm r v)
     as (R.pts_to r.r1 full_perm v.v1 `star`
         R.pts_to r.r2 full_perm v.v2);
-
-  introduce exists (v_:Ghost.erased rec_repr). (
-    pure (v == v_)
-  ) with _;
 
   rewrite (R.pts_to r.r1 full_perm v.v1 `star`
            R.pts_to r.r2 full_perm v.v2)
@@ -90,14 +93,12 @@ fn rec_get_witness (r:rec2) (#v:Ghost.erased rec_repr)
 }
 ```
 
+//Syntax for a field update on v1
 let rec_repr_with_v2 (v:rec_repr) (v2:U8.t) = { v1=v.v1; v2=v2 }
 
-// error says: could not infer implicit arguments in rec_perm on line 94,
-// but this fcn has no implicit args. also, this fcn errors at a different
-// line (88) when the remainder of this file is *not* commented out... strange
-[@@expect_failure]
+
 ```pulse
-fn mutate_rec_get_witness (r:rec2) (#v:Ghost.erased rec_repr)
+fn explicit_unfold_witness_taking_and_fold (r:rec2) (#v:Ghost.erased rec_repr)
   requires rec_perm r v
   ensures exists (v_:rec_repr) . rec_perm r v_
 {
@@ -105,12 +106,9 @@ fn mutate_rec_get_witness (r:rec2) (#v:Ghost.erased rec_repr)
     as (R.pts_to r.r1 full_perm v.v1 `star`
         R.pts_to r.r2 full_perm v.v2);
 
-  mutate_ref r.r2 0uy;
+  r.r2 := 0uy;
   let v2_ = get_witness(r.r2);
 
-
-  // assert_ (R.pts_to r.r1 full_perm v.v1 `star`
-  //          R.pts_to r.r2 full_perm v2_);
 
   rewrite (R.pts_to r.r1 full_perm v.v1 `star`
            R.pts_to r.r2 full_perm v2_)
@@ -119,73 +117,22 @@ fn mutate_rec_get_witness (r:rec2) (#v:Ghost.erased rec_repr)
 }
 ```
 
-
-(* same experiments but with records of arrays instead of byte refs *)
-
-noeq
-type rec_array = {
-  r1: A.array U8.t;
-  r2: A.array U8.t;
-}
-
-type rec_array_repr = {
-  v1: Seq.seq U8.t;
-  v2: Seq.seq U8.t;
-}
-
-let rec_array_perm (r:rec_array) (v:rec_array_repr)
-  : vprop = 
-  A.pts_to r.r1 full_perm v.v1 `star`
-  A.pts_to r.r2 full_perm v.v2
-
-// helpers 
-
 ```pulse
-fn get_witness_array (x:A.array U8.t) (#y:Ghost.erased (Seq.seq U8.t))
-requires A.pts_to x full_perm y
-returns z:Ghost.erased (Seq.seq U8.t)
-ensures A.pts_to x full_perm y ** pure (y==z)
-{   
-    y
-}
-```
-
-```pulse
-fn mutate_array (l:US.t) (a:(a:A.array U8.t{ US.v l == A.length a }))
-                (#s:(s:Ghost.erased (Seq.seq U8.t){ US.v l > 0 /\ US.v l == Seq.length s }))
-   requires A.pts_to a full_perm s
-   ensures A.pts_to a full_perm (Seq.upd s 0 0uy)
+fn explicit_unfold_slightly_better_witness_taking_and_fold (r:rec2) (#v:Ghost.erased rec_repr)
+  requires rec_perm r v
+  ensures exists (v_:rec_repr) . rec_perm r v_
 {
-  (a.(0sz) <- 0uy)
-}
-```
+  rewrite (rec_perm r v)
+    as (R.pts_to r.r1 full_perm v.v1 `star`
+        R.pts_to r.r2 full_perm v.v2);
 
+  r.r2 := 0uy;
+  with v2_. assert (R.pts_to r.r2 full_perm v2_);
 
-// same failure as mutate_rec_get_witness. suprrising that getting
-// an array witness works (line 168) because the same currently 
-// fails in L0Core.fst:232 ...
-[@@expect_failure]
-```pulse
-fn mutate_rec_get_witness (l:US.t) (r:rec_array) (#v:Ghost.erased rec_array_repr)
-  requires (
-    rec_array_perm r v `star`
-    pure (US.v l > 0 /\ A.length r.r2 == (US.v l) /\ Seq.length v.v2 == (US.v l))
-  )
-  ensures (
-    A.pts_to r.r1 full_perm v.v1 `star`
-    exists (v_:Seq.seq U8.t) . A.pts_to r.r2 full_perm v_
-  )
-{
-  rewrite (rec_array_perm r v)
-    as (A.pts_to r.r1 full_perm v.v1 `star`
-        A.pts_to r.r2 full_perm v.v2);
-  
-  mutate_array l r.r2;
-  let y = get_witness_array (r.r2); (* this works! *)
+  rewrite (R.pts_to r.r1 full_perm v.v1 `star`
+           R.pts_to r.r2 full_perm v2_)
+    as    (rec_perm r (rec_repr_with_v2 v v2_));
 
-  rewrite (A.pts_to r.r1 full_perm v.v1 `star`
-           A.pts_to r.r2 full_perm y)
-    as `@(rec_array_perm r {v with v2=y});
   ()
 }
 ```
